Split bf_resize_ok into shrink/expand ok
Each has an idiosyncratic way of stating what is preserved in
separation logic. We have yet to see what higher levels will need from
these specs, but it seems reasonable to have one spec for each of the
two modes of operation and have the application choose which one to use
(eg, by having bf_shrink and bf_expand be aliases to bf_resize with
different automation hints).

src/BFileRec.v
@@ -342,12 +342,26 @@ Section RECBFILE.
 
   (** TODO: split bf_resize into shrink/expand and give them different specs **)
 
-  Theorem bf_resize_ok : forall fsxp inum count_items mscs,
-  {< mbase m F Fm A f flist ilist,
+  (* Note: these functions are the same but have distinct nice names
+     in the context of shrinking/expanding *)
+  (** When the file is shrunk to hold count_items,
+      how many items do we actually retain? *)
+  Definition kept_items count_items : nat := roundup count_items (# items_per_valu).
+  (** When the file is expanded to hold count_items,
+      how many items do we actually allocate space for? *)
+  Definition alloc_items count_items : nat := roundup count_items (# items_per_valu).
+
+  Theorem bf_shrink_ok : forall fsxp inum count_items mscs,
+  {< mbase m F Fm A Fi f flist ilist deleted,
     PRE LOG.rep (FSXPLog fsxp) F (ActiveTxn mbase m) mscs *
     [[ (Fm * BFILE.rep (FSXPBlockAlloc fsxp) (FSXPInode fsxp) flist)%pred (list2mem m) ]] *
     [[ (A * #inum |-> f)%pred (list2nmem flist) ]] *
-    [[ array_item_file f ilist ]]
+    [[ array_item_file f ilist ]] *
+    (* split items into preserved [Fi] and [deleted] items *)
+    (* this also ensures count_items < length ilist and this is a shrink *)
+    [[ (Fi * arrayN (kept_items count_items) deleted)%pred (list2nmem ilist) ]] *
+    (* the [deleted] list is actually the rest of [ilist], not some strict prefix *)
+    [[ length deleted + kept_items count_items = length ilist ]]
     POST RET: ^(mscs, ok)
     exists m',
     LOG.rep (FSXPLog fsxp) F (ActiveTxn mbase m') mscs *
@@ -356,9 +370,37 @@ Section RECBFILE.
       [[ ok = true ]] *
       [[ (A * #inum |-> f')%pred (list2nmem flist) ]] *
       [[ array_item_file f' ilist' ]] *
-      [[ length ilist' >= count_items ]] *
-      (** TODO: need predicate saying one of ilist, ilist' is a prefix of the other **)
-      [[ firstn (length ilist) ilist' = ilist ]] )
+      (* preserves any predicate regarding the non-deleted items *)
+      (* [length ilist' <= length ilist] is implied by setting [Fi] appropriately *)
+      [[ Fi%pred (list2nmem ilist') ]] )
+    CRASH LOG.would_recover_old (FSXPLog fsxp) F mbase
+  >} bf_resize fsxp inum count_items mscs.
+  Proof.
+    unfold bf_resize.
+  Admitted.
+
+  Theorem bf_expand_ok : forall fsxp inum count_items mscs,
+  {< mbase m F Fm Fi A f flist ilist,
+   PRE LOG.rep (FSXPLog fsxp) F (ActiveTxn mbase m) mscs *
+    [[ (Fm * BFILE.rep (FSXPBlockAlloc fsxp) (FSXPInode fsxp) flist)%pred (list2mem m) ]] *
+    [[ (A * #inum |-> f)%pred (list2nmem flist) ]] *
+    [[ array_item_file f ilist ]] *
+    [[ Fi%pred (list2nmem ilist) ]] *
+    (* require that this is an expand since postcondition implies all of ilist
+       is preserved  *)
+    [[ count_items >= length ilist ]]
+    POST RET: ^(mscs, ok)
+    exists m',
+    LOG.rep (FSXPLog fsxp) F (ActiveTxn mbase m') mscs *
+      ( [[ ok = false ]] \/
+      exists f' ilist' newitems,
+      [[ ok = true ]] *
+      [[ (A * #inum |-> f')%pred (list2nmem flist) ]] *
+      [[ array_item_file f' ilist' ]] *
+      (* we don't mess with ilist ([Fi] still holds) *)
+      [[ (Fi * arrayN (length ilist) newitems)%pred (list2nmem ilist') ]] *
+      (* [length ilist' >= length ilist] is implied by setting [Fi] appropriately *)
+      [[ length newitems = alloc_items count_items - length ilist ]] )
     CRASH LOG.would_recover_old (FSXPLog fsxp) F mbase
   >} bf_resize fsxp inum count_items mscs.
   Proof.
